Progress towards partial map

LPAC_Checker/IICF_PartialMap.thy
@@ -3,6 +3,8 @@ theory IICF_PartialMap
     Isabelle_LLVM.IICF
     Isabelle_LLVM.Proto_EOArray
     Isabelle_LLVM.LLVM_DS_Block_Alloc
+    IICF_Copying_List
+    (* TODO: We only really use IICF_Copying_List for the copying setup, maybe that should live somewhere else? *)
 begin
 
 text \<open>This theory implement a key-value map.
@@ -15,10 +17,10 @@ text \<open>TODO list \<emdash> coverage of the @{theory Isabelle_LLVM.IICF_Map}
     (none yet)
 
   Missing, core operations:
-    \<^item> [ ] \<open>op_map_empty\<close>        (fresh @{term narray_assn}; slots are \<open>init = dflt = None\<close>)
-    \<^item> [ ] \<open>op_map_update\<close>       (must free the overwritten value if the key was present)
-    \<^item> [ ] \<open>op_map_delete\<close>       (must free the removed value; leaves a \<open>dflt\<close> hole)
-    \<^item> [ ] \<open>op_map_contains_key\<close> (pure; the \<open>is_dflt\<close> null test, no ownership transfer)
+    \<^item> [x] \<open>op_map_empty\<close>        (fresh @{term narray_assn}; slots are \<open>init = dflt = None\<close>)
+    \<^item> [x] \<open>op_map_update\<close>       (must free the overwritten value if the key was present)
+    \<^item> [x] \<open>op_map_delete\<close>       (must free the removed value; leaves a \<open>dflt\<close> hole)
+    \<^item> [x] \<open>op_map_contains_key\<close> (pure; the \<open>is_dflt\<close> null test, no ownership transfer)
     \<^item> [ ] \<open>op_map_is_empty\<close>     (needs a size field or a full scan)
 
   Missing, extract a value (element leaves or is copied out of the map):
@@ -52,9 +54,9 @@ definition \<open>opt_list_empty \<equiv> ([] :: 'a opt_list)\<close>
 definition \<open>opt_list_update k v m \<equiv> (m @ replicate (k + 1 - length m) None)[k:=Some v]\<close>
 definition \<open>opt_list_delete k m \<equiv> if k < length m then m[k:=None] else m\<close>
 definition \<open>opt_list_contains_key k m \<equiv> if k < length m then m!k \<noteq> None else False\<close>
-definition \<open>opt_map_is_empty \<equiv> list_all (\<lambda>x. x = None)\<close>
-definition \<open>opt_map_lookup k m \<equiv> if k < length m then m!k else None\<close>
-definition \<open>opt_map_the_lookup k m \<equiv> the (m!k)\<close>
+definition \<open>opt_list_is_empty \<equiv> list_all (\<lambda>x. x = None)\<close>
+definition \<open>opt_list_lookup k m \<equiv> if k < length m then m!k else None\<close>
+definition \<open>opt_list_the_lookup k m \<equiv> the (m!k)\<close>
 
 lemma opt_list_empty_refine:
   \<open>(uncurry0 (RETURN opt_list_empty), uncurry0 (RETURN op_map_empty))
@@ -88,23 +90,27 @@ lemma opt_list_contains_key_refine:
   apply (intro frefI nres_relI)
   by (auto simp: opt_list_map_rel_def in_br_conv opt_list_contains_key_def opt_list_\<alpha>_def dom_def)
 
-lemma opt_map_is_empty_refine:
-  \<open>(RETURN o opt_map_is_empty, RETURN o op_map_is_empty)
+lemma opt_list_is_empty_refine:
+  \<open>(RETURN o opt_list_is_empty, RETURN o op_map_is_empty)
     \<in> opt_list_map_rel \<rightarrow>\<^sub>f \<langle>bool_rel\<rangle>nres_rel\<close>
   apply (intro frefI nres_relI)
-  by (auto simp: opt_list_map_rel_def in_br_conv opt_map_is_empty_def opt_list_\<alpha>_def list_all_length fun_eq_iff)
+  by (auto simp: opt_list_map_rel_def in_br_conv opt_list_is_empty_def opt_list_\<alpha>_def list_all_length fun_eq_iff)
 
-lemma opt_map_lookup_refine:
-  \<open>(uncurry (RETURN oo opt_map_lookup), uncurry (RETURN oo op_map_lookup))
+lemma opt_list_lookup_refine:
+  \<open>(uncurry (RETURN oo opt_list_lookup), uncurry (RETURN oo op_map_lookup))
     \<in> nat_rel \<times>\<^sub>r opt_list_map_rel \<rightarrow>\<^sub>f \<langle>\<langle>Id\<rangle>option_rel\<rangle>nres_rel\<close>
   apply (intro frefI nres_relI)
-  by (auto simp: opt_list_map_rel_def in_br_conv opt_map_lookup_def opt_list_\<alpha>_def)
+  by (auto simp: opt_list_map_rel_def in_br_conv opt_list_lookup_def opt_list_\<alpha>_def)
 
-lemma opt_map_the_lookup_refine:
-  \<open>(uncurry (RETURN oo opt_map_the_lookup), uncurry (RETURN oo op_map_the_lookup))
+lemma opt_list_the_lookup_refine:
+  \<open>(uncurry (RETURN oo opt_list_the_lookup), uncurry (RETURN oo op_map_the_lookup))
     \<in> [\<lambda>(k,m). m k \<noteq> None]\<^sub>f nat_rel \<times>\<^sub>r opt_list_map_rel \<rightarrow> \<langle>Id\<rangle>nres_rel\<close>
   apply (intro frefI nres_relI)
-  by (auto simp: opt_list_map_rel_def in_br_conv opt_map_the_lookup_def opt_list_\<alpha>_def split: if_splits)
+  by (auto simp: opt_list_map_rel_def in_br_conv opt_list_the_lookup_def opt_list_\<alpha>_def split: if_splits)
+
+lemma opt_list_contains_key_fcomp[fcomp_prenorm_simps]:
+  \<open>(ol, m) \<in> opt_list_map_rel \<Longrightarrow> opt_list_contains_key k ol \<longleftrightarrow> m k \<noteq> None\<close>
+  by (auto simp: opt_list_map_rel_def in_br_conv opt_list_contains_key_def opt_list_\<alpha>_def)
 
 section \<open>Low-level implementation\<close>
 text \<open>Now we implement our option list on llvm level.\<close>
@@ -113,19 +119,24 @@ subsection \<open>Init-tailed array list\<close>
 text \<open>@{term arl_assn} does not fill the tail with @{term init} on resize, so we'd have to initialize
   each element. Therefore we define a new init array list and reuse @{term arl_assn} where possible.\<close>
 
-definition iarl_assn :: \<open>('a::llvm_rep list, ('a,'l::len2) array_list) dr_assn\<close> where
+definition iarl_assn :: \<open>('a::llvm_rep list, ('a,64) array_list) dr_assn\<close> where
   \<open>iarl_assn \<equiv> mk_assn (\<lambda>xs (li,ci,ai). EXS c a.
       \<upharpoonleft>snat.assn (length xs) li ** \<upharpoonleft>snat.assn c ci ** \<upharpoonleft>narray_assn a ai
-      ** \<up>(4 < LENGTH('l) \<and> length xs \<le> c \<and> c = length a
+      ** \<up>(length xs \<le> c \<and> c = length a
             \<and> a = xs @ replicate (c - length xs) init))\<close>
 
+lemma snat8_64[simp]: \<open>8 \<in> snats LENGTH(64)\<close>
+  by (simp add: snats_def)
+
 lemma iarl_new_raw_rule[vcg_rules]:
-  \<open>llvm_htriple (\<up>(4 < LENGTH('l)))
-     (arl_new_raw :: ('a::llvm_rep,'l::len2) array_list llM)
+  \<open>llvm_htriple \<box>
+     (arl_new_raw :: ('a::llvm_rep,64) array_list llM)
      (\<lambda>r. \<upharpoonleft>iarl_assn ([]::'a list) r)\<close>
   unfolding arl_new_raw_def arl_initial_size_def iarl_assn_def
   apply (vcg_monadify)
-  by vcg'
+  apply vcg'
+  by (metis snat8_64)
+  
 
 lemma iarl_len_rule[vcg_rules]:
   \<open>llvm_htriple (\<upharpoonleft>iarl_assn xs ali) (arl_len ali)
@@ -149,7 +160,7 @@ lemma iarl_upd_rule[vcg_rules]:
   unfolding iarl_assn_def arl_upd_def
   by vcg
 
-definition iarl_resize :: \<open>'l word \<Rightarrow> ('a::llvm_rep, 'l::len2) array_list \<Rightarrow> ('a, 'l) array_list llM\<close> where[llvm_code]:
+definition iarl_resize :: \<open>64 word \<Rightarrow> ('a::llvm_rep, 64) array_list \<Rightarrow> ('a, 64) array_list llM\<close> where[llvm_code]:
   \<open>iarl_resize c' al \<equiv> doM {
     al \<leftarrow> arl_ensure_capacity c' al;  
     let (_, c, a) = al;
@@ -190,43 +201,923 @@ definition \<open>pmap_assn \<equiv> mk_assn (\<lambda>xs (p :: (_, 64) array_li
 abbreviation \<open>pmap_assn' \<equiv> \<upharpoonleft>pmap_assn\<close>
 type_synonym 'c pmap_conc = \<open>('c, 64) array_list\<close>
 
-lemma pmap_empty_hnr[sepref_fr_rules]:
+text \<open>Basic simplifications of the locale's option assertion.\<close>
+
+lemma option_assn_dflt[simp]: \<open>option_assn Option.None dflt = \<box>\<close>
+  unfolding option_assn_def by (auto simp: sep_algebra_simps)
+
+lemma option_assn_Some[simp]: \<open>option_assn (Option.Some x) c = A x c\<close>
+  unfolding option_assn_def
+  by (cases \<open>c = dflt\<close>) (auto simp: UU sep_algebra_simps)
+
+lemma option_assn_None_conv: \<open>option_assn Option.None c = \<up>(c = dflt)\<close>
+  unfolding option_assn_def by (auto simp: sep_algebra_simps)
+
+lemma list_assn_option_replicate[simp]:
+  \<open>\<upharpoonleft>(list_assn (mk_assn option_assn)) (replicate n Option.None) (replicate n init) = \<box>\<close>
+  by (induction n) (auto simp: dflt_is_init[symmetric] sep_algebra_simps)
+
+lemma list_assn_option_focus:
+  assumes A: \<open>i < length xs\<close>
+  shows \<open>\<upharpoonleft>(list_assn (mk_assn option_assn)) xs xsi =
+    (option_assn (xs!i) (xsi!i) **
+    \<upharpoonleft>(list_assn (mk_assn option_assn)) (xs[i := Option.None]) (xsi[i := dflt]))\<close>
+proof (cases \<open>length xsi = length xs\<close>)
+  case True
+  obtain xs\<^sub>1 x xs\<^sub>2 where XSF: \<open>xs = xs\<^sub>1 @ x # xs\<^sub>2\<close> and LEN1: \<open>i = length xs\<^sub>1\<close>
+    using id_take_nth_drop[OF A] A by fastforce
+  obtain ys\<^sub>1 y ys\<^sub>2 where YSF: \<open>xsi = ys\<^sub>1 @ y # ys\<^sub>2\<close> and LEN2: \<open>length ys\<^sub>1 = length xs\<^sub>1\<close>
+      and \<open>length ys\<^sub>2 = length xs\<^sub>2\<close>
+    using split_list_according[OF XSF True] .
+  show ?thesis
+    unfolding XSF YSF LEN1
+    by (simp add: LEN2 nth_append list_update_append sep_algebra_simps sep_conj_c)
+next
+  case False
+  then show ?thesis by simp
+qed
+
+lemma list_assn_option_insert:
+  assumes \<open>i < length xs\<close>
+  shows \<open>\<upharpoonleft>(list_assn (mk_assn option_assn)) (xs[i := Option.Some v]) (xsi[i := vi]) =
+    (A v vi ** \<upharpoonleft>(list_assn (mk_assn option_assn)) (xs[i := Option.None]) (xsi[i := dflt]))\<close>
+proof (cases \<open>i < length xsi\<close>)
+  case True
+  from assms have \<open>i < length (xs[i := Option.Some v])\<close> by simp
+  from list_assn_option_focus[OF this, of \<open>xsi[i := vi]\<close>] show ?thesis
+    using assms True by simp
+next
+  case False
+  then show ?thesis using assms by (simp add: sep_algebra_simps)
+qed
+
+lemma pmap_empty_hnr:
   \<open>(uncurry0 arl_new_raw, uncurry0 (RETURN opt_list_empty)) \<in> unit_assn\<^sup>k \<rightarrow>\<^sub>a pmap_assn'\<close>
   supply [simp] = pmap_assn_def opt_list_empty_def
   by (sepref_to_hoare; vcg)
 
+lemmas pmap_empty_hnr2[sepref_fr_rules] =
+  pmap_empty_hnr[FCOMP opt_list_empty_refine]
+
+lemma pmap_free_slot_rule[vcg_rules]:
+  \<open>llvm_htriple
+     (\<upharpoonleft>(list_assn (mk_assn option_assn)) xs xsi ** \<up>\<^sub>d(i < length xs))
+     (free_option afree (xsi ! i))
+     (\<lambda>_. \<upharpoonleft>(list_assn (mk_assn option_assn)) (xs[i := Option.None]) (xsi[i := dflt]))\<close>
+proof (cases \<open>i < length xs\<close>)
+  case True
+  show ?thesis
+    supply [vcg_rules] = mk_free_option[OF Afree, THEN MK_FREED]
+    unfolding vcg_tag_defs list_assn_option_focus[OF True]
+    by vcg
+next
+  case False
+  show ?thesis
+    unfolding vcg_tag_defs
+    apply (rule htriple_realizable_preI)
+    using False by (simp add: sep_algebra_simps)
+qed
+
 (* note that our update takes ownership *)
 definition pmap_update :: \<open>64 word \<Rightarrow> 'a \<Rightarrow> 'a pmap_conc \<Rightarrow> 'a pmap_conc llM\<close> where[llvm_code]:
   \<open>pmap_update ki vi ai \<equiv> doM {
-    l \<leftarrow> arl_len ai; 
-    if (ki < l) then doM {
+    l \<leftarrow> arl_len ai;
+    b \<leftarrow> ll_icmp_ult ki l;
+    llc_if b (doM {
       prev \<leftarrow> arl_nth ai ki;
       free_option afree prev;
       arl_upd ai ki vi
-    } else doM {
-      ai \<leftarrow> iarl_resize (ki + 1) ai;
-      arl_upd ai ki vi 
-    }
+    }) (doM {
+      k1 \<leftarrow> ll_add ki 1;
+      ai \<leftarrow> iarl_resize k1 ai;
+      arl_upd ai ki vi
+    })
   }\<close>
 
+lemma pmap_update_reassemble_present:
+  assumes A: \<open>k < length xsi\<close>
+  shows \<open>ENTAILS
+    (\<upharpoonleft>iarl_assn (xsi[k := vi]) ai **
+     \<upharpoonleft>(list_assn (mk_assn option_assn)) (xs[k := Option.None]) (xsi[k := dflt]) ** A v vi)
+    (EXS z. \<upharpoonleft>iarl_assn z ai **
+       \<upharpoonleft>(list_assn (mk_assn option_assn))
+          ((xs @ replicate (Suc k - length xs) Option.None)[k := Option.Some v]) z)\<close>
+proof (cases \<open>length xs = length xsi\<close>)
+  case True
+  with A have K: \<open>k < length xs\<close> by simp
+  then have [simp]: \<open>Suc k - length xs = 0\<close> by simp
+  show ?thesis
+    unfolding ENTAILS_def
+    apply simp
+    apply (rule entails_exI[where x=\<open>xsi[k := vi]\<close>])
+    by (simp add: list_assn_option_insert[OF K] sep_conj_aci)
+next
+  case False
+  then show ?thesis
+    unfolding ENTAILS_def by (auto simp: entails_def sep_algebra_simps)
+qed
+
+lemma pmap_update_reassemble_absent:
+  assumes A: \<open>\<not> k < length xsi\<close>
+  shows \<open>ENTAILS
+    (\<upharpoonleft>iarl_assn ((xsi @ replicate (Suc k - length xsi) init)[k := vi]) ai **
+     \<upharpoonleft>(list_assn (mk_assn option_assn)) xs xsi ** A v vi)
+    (EXS z. \<upharpoonleft>iarl_assn z ai **
+       \<upharpoonleft>(list_assn (mk_assn option_assn))
+          ((xs @ replicate (Suc k - length xs) Option.None)[k := Option.Some v]) z)\<close>
+proof (cases \<open>length xs = length xsi\<close>)
+  case True
+  with A have LE: \<open>length xs \<le> k\<close> by simp
+  have K: \<open>k < length (xs @ replicate (Suc k - length xs) Option.None)\<close>
+    using LE by simp
+  have 1: \<open>(xs @ replicate (Suc k - length xs) Option.None)[k := Option.None]
+         = xs @ replicate (Suc k - length xs) Option.None\<close>
+    using LE by (simp add: list_update_append list_update_same_conv)
+  have 2: \<open>(xsi @ replicate (Suc k - length xsi) init)[k := dflt]
+         = xsi @ replicate (Suc k - length xsi) init\<close>
+    using A by (simp add: list_update_append list_update_same_conv dflt_is_init)
+  have 3: \<open>\<upharpoonleft>(list_assn (mk_assn option_assn)) (xs @ replicate (Suc k - length xs) Option.None)
+             (xsi @ replicate (Suc k - length xsi) init)
+         = \<upharpoonleft>(list_assn (mk_assn option_assn)) xs xsi\<close>
+    using True by (simp add: sep_algebra_simps)
+  show ?thesis
+    unfolding ENTAILS_def
+    apply (rule entails_exI[where x=\<open>(xsi @ replicate (Suc k - length xsi) init)[k := vi]\<close>])
+    by (simp add: list_assn_option_insert[OF K] 1 2 3 sep_conj_aci)
+next
+  case False
+  then show ?thesis
+    unfolding ENTAILS_def by (auto simp: entails_def sep_algebra_simps)
+qed
+
+
 lemma pmap_update_rule[vcg_rules]:
-  \<open>k < max_snat 64 \<Longrightarrow> llvm_htriple
-    (\<upharpoonleft>snat.assn k ki ** A v vi ** pmap_assn' xs ai)
+  \<open>llvm_htriple
+    (\<upharpoonleft>snat.assn k ki ** A v vi ** pmap_assn' xs ai ** \<up>\<^sub>d(k + 1 < max_snat 64))
     (pmap_update ki vi ai)
-    (\<lambda>ai'. pmap_assn' (xs[k:=Some v]) ai')\<close>
-  unfolding pmap_update_def 
+    (\<lambda>ai'. pmap_assn' (opt_list_update k v xs) ai')\<close>
+  unfolding pmap_update_def opt_list_update_def
+  supply [simp] = pmap_assn_def list_assn_option_focus
+  apply vcg
+  subgoal by (rule pmap_update_reassemble_present)
+  apply vcg
+  subgoal by (rule pmap_update_reassemble_absent)
+  done
+
+lemma pmap_update_hnr:
+  \<open>(uncurry2 pmap_update, uncurry2 (RETURN ooo opt_list_update))
+    \<in> [\<lambda>((k,_),_). k + 1 < max_snat 64]\<^sub>a
+      (snat_assn' TYPE(64))\<^sup>k *\<^sub>a A\<^sup>d *\<^sub>a pmap_assn'\<^sup>d \<rightarrow> pmap_assn'\<close>
+  unfolding snat_rel_def snat.assn_is_rel[symmetric]
+  apply sepref_to_hoare
+  by vcg
+
+lemmas pmap_update_hnr2[sepref_fr_rules] =
+  pmap_update_hnr[FCOMP opt_list_update_refine]
+
+definition pmap_delete :: \<open>64 word \<Rightarrow> 'a pmap_conc \<Rightarrow> 'a pmap_conc llM\<close> where[llvm_code]:
+  \<open>pmap_delete ii ai \<equiv> doM {
+    l \<leftarrow> arl_len ai;
+    cmp \<leftarrow> ll_icmp_ult ii l;
+    llc_if cmp (doM {
+      prev \<leftarrow> arl_nth ai ii;
+      free_option afree prev;
+      arl_upd ai ii init
+    })
+    (Mreturn ai)
+  }\<close>
+
+lemma pmap_delete_reassemble_present:
+  assumes A: \<open>k < length xsi\<close>
+  shows \<open>ENTAILS
+    (\<upharpoonleft>iarl_assn (xsi[k := dflt]) ai **
+     \<upharpoonleft>(list_assn (mk_assn option_assn)) (xs[k := Option.None]) (xsi[k := dflt]))
+    (EXS z. \<upharpoonleft>iarl_assn z ai **
+       \<upharpoonleft>(list_assn (mk_assn option_assn)) (if k < length xs then xs[k := Option.None] else xs) z)\<close>
+proof (cases \<open>length xs = length xsi\<close>)
+  case True
+  with A have [simp]: \<open>k < length xs\<close> by simp
+  show ?thesis
+    unfolding ENTAILS_def
+    apply simp
+    apply (rule entails_exI[where x=\<open>xsi[k := dflt]\<close>])
+    by (simp add: entails_refl)
+next
+  case False
+  then show ?thesis
+    unfolding ENTAILS_def by (auto simp: entails_def sep_algebra_simps)
+qed
+
+lemma pmap_delete_reassemble_absent:
+  assumes A: \<open>\<not> k < length xsi\<close>
+  shows \<open>ENTAILS
+    (\<upharpoonleft>iarl_assn xsi ai ** \<upharpoonleft>(list_assn (mk_assn option_assn)) xs xsi)
+    (EXS z. \<upharpoonleft>iarl_assn z ai **
+       \<upharpoonleft>(list_assn (mk_assn option_assn)) (if k < length xs then xs[k := Option.None] else xs) z)\<close>
+proof (cases \<open>length xs = length xsi\<close>)
+  case True
+  with A have [simp]: \<open>\<not> k < length xs\<close> by simp
+  show ?thesis
+    unfolding ENTAILS_def
+    apply simp
+    apply (rule entails_exI[where x=xsi])
+    by (simp add: entails_refl)
+next
+  case False
+  then show ?thesis
+    unfolding ENTAILS_def by (auto simp: entails_def sep_algebra_simps)
+qed
+
+lemma pmap_delete_rule[vcg_rules]:
+  \<open>llvm_htriple
+    (\<upharpoonleft>snat.assn k ki ** pmap_assn' xs ai)
+    (pmap_delete ki ai)
+    (\<lambda>ai'. pmap_assn' (opt_list_delete k xs) ai')\<close>
+  unfolding pmap_delete_def opt_list_delete_def
+  supply [simp] = pmap_assn_def dflt_is_init[symmetric]
+  apply vcg
+  subgoal by (rule pmap_delete_reassemble_present)
+  apply vcg
+  subgoal by (rule pmap_delete_reassemble_absent)
+  done
+
+lemma pmap_delete_hnr:
+  \<open>(uncurry pmap_delete, uncurry (RETURN oo opt_list_delete))
+    \<in> (snat_assn' TYPE(64))\<^sup>k *\<^sub>a pmap_assn'\<^sup>d \<rightarrow>\<^sub>a pmap_assn'\<close>
+  unfolding snat_rel_def snat.assn_is_rel[symmetric]
+  apply sepref_to_hoare
+  by vcg
+
+lemmas pmap_delete_hnr2[sepref_fr_rules] =
+  pmap_delete_hnr[FCOMP opt_list_delete_refine]
+
+lemma A_ne_dflt_conv: \<open>A a c = (\<up>(c \<noteq> dflt) ** A a c)\<close>
+  by (cases \<open>c = dflt\<close>) (auto simp: UU sep_algebra_simps)
+
+lemma pmap_is_dflt_rule[vcg_rules]:
+  \<open>llvm_htriple
+     (\<upharpoonleft>(list_assn (mk_assn option_assn)) xs xsi ** \<up>\<^sub>d(i < length xs))
+     (is_dflt (xsi ! i))
+     (\<lambda>r. \<upharpoonleft>(list_assn (mk_assn option_assn)) xs xsi ** \<upharpoonleft>bool.assn (xs ! i = Option.None) r)\<close>
+proof (cases \<open>i < length xs\<close>)
+  case True
+  note F = list_assn_option_focus[OF True]
+  show ?thesis
+  proof (cases \<open>xs ! i\<close>)
+    case None
+    show ?thesis
+      supply [vcg_rules] = CMP
+      unfolding vcg_tag_defs F None option_assn_None_conv
+      by vcg
+  next
+    case (Some y)
+    show ?thesis
+      supply [vcg_rules] = CMP
+      unfolding vcg_tag_defs F Some option_assn_Some
+      apply (subst A_ne_dflt_conv)
+      by vcg
+  qed
+next
+  case False
+  show ?thesis
+    unfolding vcg_tag_defs
+    apply (rule htriple_realizable_preI)
+    using False by (simp add: sep_algebra_simps)
+qed
+
+definition pmap_contains_key :: \<open>64 word \<Rightarrow> 'a pmap_conc \<Rightarrow> 1 word llM\<close> where[llvm_code]:
+  \<open>pmap_contains_key ii ai \<equiv> doM {
+    l \<leftarrow> arl_len ai;
+    isin \<leftarrow> ll_icmp_ult ii l;
+    llc_if isin (doM {
+      item \<leftarrow> arl_nth ai ii;
+      d \<leftarrow> is_dflt item;
+      llc_if d (Mreturn 0) (Mreturn 1)
+    })
+    (Mreturn 0)
+  }\<close>
+
+lemma pmap_contains_key_reassemble_absent_slot:
+  assumes A: \<open>k < length xsi\<close> and B: \<open>xs ! k = Option.None\<close>
+  shows \<open>ENTAILS
+    (\<upharpoonleft>(list_assn (mk_assn option_assn)) xs xsi ** \<upharpoonleft>iarl_assn xsi ai)
+    ((EXS z. \<upharpoonleft>iarl_assn z ai ** \<upharpoonleft>(list_assn (mk_assn option_assn)) xs z)
+      ** \<upharpoonleft>bool.assn (if k < length xs then xs ! k \<noteq> Option.None else False) 0)\<close>
+proof (cases \<open>length xs = length xsi\<close>)
+  case True
+  with A have [simp]: \<open>k < length xs\<close> by simp
+  show ?thesis
+    unfolding ENTAILS_def
+    apply (simp add: B bool.assn_def sep_algebra_simps)
+    apply (rule entails_exI[where x=xsi])
+    by (simp add: sep_conj_aci entails_refl)
+next
+  case False
+  then show ?thesis
+    unfolding ENTAILS_def by (auto simp: entails_def sep_algebra_simps)
+qed
+
+lemma pmap_contains_key_reassemble_present_slot:
+  assumes A: \<open>k < length xsi\<close> and B: \<open>xs ! k = Option.Some y\<close>
+  shows \<open>ENTAILS
+    (\<upharpoonleft>(list_assn (mk_assn option_assn)) xs xsi ** \<upharpoonleft>iarl_assn xsi ai)
+    ((EXS z. \<upharpoonleft>iarl_assn z ai ** \<upharpoonleft>(list_assn (mk_assn option_assn)) xs z)
+      ** \<upharpoonleft>bool.assn (if k < length xs then xs ! k \<noteq> Option.None else False) 1)\<close>
+proof (cases \<open>length xs = length xsi\<close>)
+  case True
+  with A have [simp]: \<open>k < length xs\<close> by simp
+  show ?thesis
+    unfolding ENTAILS_def
+    apply (simp add: B bool.assn_def sep_algebra_simps)
+    apply (rule entails_exI[where x=xsi])
+    by (simp add: sep_conj_aci entails_refl)
+next
+  case False
+  then show ?thesis
+    unfolding ENTAILS_def by (auto simp: entails_def sep_algebra_simps)
+qed
+
+lemma pmap_contains_key_reassemble_oob:
+  assumes A: \<open>\<not> k < length xsi\<close>
+  shows \<open>ENTAILS
+    (\<upharpoonleft>iarl_assn xsi ai ** \<upharpoonleft>(list_assn (mk_assn option_assn)) xs xsi)
+    ((EXS z. \<upharpoonleft>iarl_assn z ai ** \<upharpoonleft>(list_assn (mk_assn option_assn)) xs z)
+      ** \<upharpoonleft>bool.assn (if k < length xs then xs ! k \<noteq> Option.None else False) 0)\<close>
+proof (cases \<open>length xs = length xsi\<close>)
+  case True
+  with A have [simp]: \<open>\<not> k < length xs\<close> by simp
+  show ?thesis
+    unfolding ENTAILS_def
+    apply (simp add: bool.assn_def sep_algebra_simps)
+    apply (rule entails_exI[where x=xsi])
+    by (simp add: sep_conj_aci entails_refl)
+next
+  case False
+  then show ?thesis
+    unfolding ENTAILS_def by (auto simp: entails_def sep_algebra_simps)
+qed
+
+lemma pmap_contains_key_rule[vcg_rules]:
+  \<open>llvm_htriple
+    (\<upharpoonleft>snat.assn k ki ** pmap_assn' xs ai)
+    (pmap_contains_key ki ai)
+    (\<lambda>r. pmap_assn' xs ai ** \<upharpoonleft>bool.assn (opt_list_contains_key k xs) r)\<close>
+  unfolding pmap_contains_key_def opt_list_contains_key_def
   supply [simp] = pmap_assn_def
-  apply (cases \<open>ki < l\<close>)
-  subgoal
+  apply vcg
+  subgoal by (rule pmap_contains_key_reassemble_absent_slot)
+  apply vcg
+  subgoal by (rule pmap_contains_key_reassemble_present_slot)
+  apply vcg
+  subgoal by (rule pmap_contains_key_reassemble_oob)
+  done
+
+lemma pmap_contains_key_hnr:
+  \<open>(uncurry pmap_contains_key, uncurry (RETURN oo opt_list_contains_key))
+    \<in> (snat_assn' TYPE(64))\<^sup>k *\<^sub>a pmap_assn'\<^sup>k \<rightarrow>\<^sub>a bool1_assn\<close>
+  unfolding snat_rel_def snat.assn_is_rel[symmetric]
+    bool1_rel_def bool.assn_is_rel[symmetric]
+  apply sepref_to_hoare
+  by vcg
+
+lemmas pmap_contains_key_hnr2[sepref_fr_rules] =
+  pmap_contains_key_hnr[FCOMP opt_list_contains_key_refine]
+
+lemma pmap_lookup_reassemble_present:
+  assumes A: \<open>k < length xsi\<close>
+  shows \<open>ENTAILS
+    (\<upharpoonleft>iarl_assn (xsi[k := dflt]) ai ** \<upharpoonleft>(list_assn (mk_assn option_assn)) xs xsi)
+    ((EXS z. \<upharpoonleft>iarl_assn z ai **
+        \<upharpoonleft>(list_assn (mk_assn option_assn)) (xs[k := Option.None]) z)
+     ** option_assn (if k < length xs then xs ! k else Option.None) (xsi ! k))\<close>
+proof (cases \<open>length xs = length xsi\<close>)
+  case True
+  with A have K: \<open>k < length xs\<close> by simp
+  show ?thesis
+    unfolding ENTAILS_def
+    apply (simp add: K list_assn_option_focus[OF K] sep_conj_exists)
+    apply (rule entails_exI[where x=\<open>xsi[k := dflt]\<close>])
+    by (simp add: sep_conj_aci entails_refl)
+next
+  case False
+  then show ?thesis
+    unfolding ENTAILS_def by (auto simp: entails_def sep_algebra_simps)
+qed
+
+lemma pmap_lookup_reassemble_oob:
+  assumes A: \<open>\<not> k < length xsi\<close>
+  shows \<open>ENTAILS
+    (\<upharpoonleft>iarl_assn xsi ai ** \<upharpoonleft>(list_assn (mk_assn option_assn)) xs xsi)
+    ((EXS z. \<upharpoonleft>iarl_assn z ai **
+        \<upharpoonleft>(list_assn (mk_assn option_assn)) (xs[k := Option.None]) z)
+     ** option_assn (if k < length xs then xs ! k else Option.None) dflt)\<close>
+proof (cases \<open>length xs = length xsi\<close>)
+  case True
+  with A have K: \<open>\<not> k < length xs\<close> by simp
+  then have K2: \<open>length xs \<le> k\<close> by simp
+  show ?thesis
+    unfolding ENTAILS_def
+    apply (simp add: K list_update_beyond[OF K2] sep_conj_exists)
+    apply (rule entails_exI[where x=xsi])
+    by (simp add: sep_conj_aci entails_refl)
+next
+  case False
+  then show ?thesis
+    unfolding ENTAILS_def by (auto simp: entails_def sep_algebra_simps)
+qed
+
+definition pmap_lookup :: \<open>64 word \<Rightarrow> 'a pmap_conc \<Rightarrow> 'a llM\<close> where[llvm_code]:
+  \<open>pmap_lookup ii ai \<equiv> doM {
+    l \<leftarrow> arl_len ai;
+    b \<leftarrow> ll_icmp_ult ii l;
+    llc_if b (doM {
+      a \<leftarrow> arl_nth ai ii;
+      arl_upd ai ii init;
+      Mreturn a
+    })
+    (Mreturn init)
+  }\<close>
+
+lemma pmap_lookup_rule[vcg_rules]:
+  \<open>llvm_htriple
+    (\<upharpoonleft>snat.assn i ii ** pmap_assn' xs ai)
+    (pmap_lookup ii ai)
+    (\<lambda>r. pmap_assn' (xs[i := Option.None]) ai ** option_assn (opt_list_lookup i xs) r)\<close>
+  unfolding pmap_lookup_def opt_list_lookup_def
+  supply [simp] = pmap_assn_def dflt_is_init[symmetric]
+  apply vcg
+  subgoal by (rule pmap_lookup_reassemble_present)
+  apply vcg
+  subgoal by (rule pmap_lookup_reassemble_oob)
+  done
+
+(* it is questionably, whether this function will ever be useful,
+ * unless sepref has some way of recognizing that the map is still
+ * alive (but with a hole) *)
+lemma pmap_lookup_opt_list_lookup:
+  \<open>(uncurry pmap_lookup, uncurry (RETURN oo opt_list_lookup))
+  \<in> (snat_assn' TYPE(64))\<^sup>k *\<^sub>a pmap_assn'\<^sup>d \<rightarrow>\<^sub>a option_assn\<close>
+  apply sepref_to_hoare
+  unfolding snat_rel_def snat.rel_def in_br_conv
+  apply vcg
+  oops (* Not sure if we even want to finish this one... *)
+
+definition pmap_free :: \<open>'a pmap_conc \<Rightarrow> unit llM\<close> where[llvm_code]:
+  \<open>pmap_free ai \<equiv> doM {
+    llc_while
+      (\<lambda>i. doM{ l \<leftarrow> arl_len ai; ll_icmp_ult i l})
+      (\<lambda>i. doM {
+        x \<leftarrow> arl_nth ai i;
+        free_option afree x; 
+        arl_upd ai i init;
+        i \<leftarrow> ll_add i (signed_nat 1);
+        Mreturn i
+      }) (signed_nat 0);
+    arl_free ai
+  }\<close>
+
+lemma iarl_free_rule[vcg_rules]: \<open>llvm_htriple (\<upharpoonleft>iarl_assn a c) (arl_free c) (\<lambda>_. \<box>)\<close>
+  unfolding iarl_assn_def arl_free_def
+  by vcg
+
+lemma iarl_free_rl[sepref_frame_free_rules]: \<open>MK_FREE (\<upharpoonleft>iarl_assn) arl_free\<close>
+  apply rule
+  by (rule iarl_free_rule)
+
+definition \<open>nulled_prefix (xs :: 'c option list) i = replicate i None @ drop i xs\<close>
+
+lemma nulled_emp[simp]: \<open>nulled_prefix xs 0 = xs\<close>
+  unfolding nulled_prefix_def by simp
+
+lemma nulled_prefix_length[simp]:
+  \<open>i \<le> length xs \<Longrightarrow> length (nulled_prefix xs i) = length xs\<close>
+  unfolding nulled_prefix_def by simp 
+
+lemma nulled_prefix_nth[simp]:
+  \<open>i < length xs \<Longrightarrow> nulled_prefix xs i ! i = xs ! i\<close>
+  unfolding nulled_prefix_def
+  by (metis Cons_nth_drop_Suc drop_append_miracle length_replicate nth_via_drop)
+
+lemma nulled_prefix_step[simp]:
+  \<open>i < length xs \<Longrightarrow> (nulled_prefix xs i)[i := Option.None] = nulled_prefix xs (Suc i)\<close>
+  unfolding nulled_prefix_def
+  by (metis Cons_nth_drop_Suc append_Cons fold_None length_replicate
+            list_update_length replicate_Suc replicate_app_Cons_same)
+
+lemma nulled_prefix_full[simp]:
+  \<open>nulled_prefix xs (length xs) = replicate (length xs) Option.None\<close>
+  unfolding nulled_prefix_def by simp
+
+lemma list_assn_option_all_None:
+  \<open>\<upharpoonleft>(list_assn (mk_assn option_assn)) (replicate n Option.None) xsi = \<up>(xsi = replicate n dflt)\<close>
+  apply (induction n arbitrary: xsi; simp)
+  by (auto simp: sep_algebra_simps list_assn_cons1_conv option_assn_None_conv)
+
+lemma pmap_free_reassemble_step:
+  assumes A: \<open>x < length xsi\<close>
+      and B: \<open>x \<le> length xs\<close>
+      and RD: \<open>\<flat>\<^sub>psnat.assn (Suc x) rd\<close>
+  shows \<open>ENTAILS
+    (\<upharpoonleft>iarl_assn (xsi[x := dflt]) ai **
+     \<upharpoonleft>(list_assn (mk_assn option_assn)) ((nulled_prefix xs x)[x := Option.None]) (xsi[x := dflt]))
+    (EXS t. (EXS i xsi'.
+        \<upharpoonleft>snat.assn i rd ** \<upharpoonleft>iarl_assn xsi' ai **
+        \<upharpoonleft>(list_assn (mk_assn option_assn)) (nulled_prefix xs i) xsi' **
+        \<up>(i \<le> length xs) ** \<up>\<^sub>!(t = length xs - i)) **
+      \<up>\<^sub>d((t, length xs - x) \<in> less_than) ** \<box>)\<close>
+proof (cases \<open>length xs = length xsi\<close>)
+  case True
+  with A have K: \<open>x < length xs\<close> by simp
+  then have K2: \<open>Suc x \<le> length xs\<close> and K3: \<open>length xs - Suc x < length xs - x\<close>
+    by arith+
+  show ?thesis
+    unfolding ENTAILS_def vcg_tag_defs
+    apply (simp add: sep_conj_exists)
+    apply (rule entails_exI[where x=\<open>length xs - Suc x\<close>])
+    apply (rule entails_exI[where x=\<open>Suc x\<close>])
+    apply (rule entails_exI[where x=\<open>xsi[x := dflt]\<close>])
+    using RD K K2 K3
+    by (simp add: snat.assn_pure[THEN extract_pure_assn]
+                  sep_algebra_simps pred_lift_extract_simps)
+next
+  case False
+  with B have \<open>length ((nulled_prefix xs x)[x := Option.None]) \<noteq> length (xsi[x := dflt])\<close>
+    by simp
+  then show ?thesis
+    unfolding ENTAILS_def by (auto simp: entails_def sep_algebra_simps)
+qed
+
+lemma pmap_free_reassemble_exit:
+  assumes A: \<open>\<not> x < length xsi\<close>
+      and B: \<open>x \<le> length xs\<close>
+  shows \<open>ENTAILS (\<upharpoonleft>(list_assn (mk_assn option_assn)) (nulled_prefix xs x) xsi) \<box>\<close>
+proof (cases \<open>length xs = length xsi\<close>)
+  case True
+  with A B have X: \<open>x = length xs\<close> by simp
+  show ?thesis
+    unfolding ENTAILS_def
+    by (simp add: X list_assn_option_all_None entails_def
+                  sep_algebra_simps pred_lift_extract_simps)
+next
+  case False
+  with B have \<open>length (nulled_prefix xs x) \<noteq> length xsi\<close> by simp
+  then show ?thesis
+    unfolding ENTAILS_def by (auto simp: entails_def sep_algebra_simps)
+qed
+
+lemma pmap_free_rule[sepref_frame_free_rules]: \<open>MK_FREE pmap_assn' pmap_free\<close>
+  apply rule
+  unfolding pmap_free_def
+  subgoal for xs ai
+    apply (rewrite annotate_llc_while[where
+    I="\<lambda>ii t. EXS i xsi. \<upharpoonleft>snat.assn i ii
+      ** \<upharpoonleft>iarl_assn xsi ai
+      ** \<upharpoonleft>(list_assn (mk_assn option_assn)) (nulled_prefix xs i) xsi
+      ** \<up>(i\<le>length xs)
+      ** \<up>\<^sub>!(t = length xs - i )"
+    and R="less_than"
+    ])
+    supply [simp] = pmap_assn_def dflt_is_init[symmetric]
+    apply vcg_monadify
     apply vcg
-    sorry
-  subgoal
+    subgoal by (rule pmap_free_reassemble_step)
     apply vcg
-    sorry
+    subgoal by (rule pmap_free_reassemble_exit)
+    done
   done
 
 end
 
-definition \<open>box_assn A \<equiv> mk_assn (\<lambda>x p. EXS c. \<upharpoonleft>ll_bpto p c ** A x c)\<close>
+section \<open>Boxing\<close>
+text \<open>To actually put arbitrary (impure) objects into our pmaps, we need to wrap them.\<close>
+
+definition box_assn :: \<open>('a \<Rightarrow> 'c::llvm_rep \<Rightarrow> assn) \<Rightarrow> ('a, 'c ptr) dr_assn\<close> where
+  \<open>box_assn A \<equiv> mk_assn (\<lambda>x p. EXS c. \<upharpoonleft>ll_bpto c p ** A x c)\<close>
+
+lemma box_assn_null[simp]: \<open>\<upharpoonleft>(box_assn A) x null = sep_false\<close>
+  unfolding box_assn_def by (auto simp: sep_algebra_simps)
+
+subsection \<open>Operations\<close>
+
+definition box_new :: \<open>'c::llvm_rep \<Rightarrow> 'c ptr llM\<close> where [llvm_code, llvm_inline]:
+  \<open>box_new c \<equiv> ll_ref c\<close>
+
+lemma box_new_rule[vcg_rules]:
+  \<open>llvm_htriple (A x c) (box_new c) (\<lambda>p. \<upharpoonleft>(box_assn A) x p)\<close>
+  unfolding box_new_def box_assn_def by vcg
+
+definition box_open :: \<open>'c::llvm_rep ptr \<Rightarrow> 'c llM\<close> where [llvm_code]:
+  \<open>box_open p \<equiv> doM {
+    c \<leftarrow> ll_load p;
+    ll_free p;
+    Mreturn c
+  }\<close>
+
+lemma box_open_rule[vcg_rules]:
+  \<open>llvm_htriple (\<upharpoonleft>(box_assn A) x p) (box_open p) (\<lambda>c. A x c)\<close>
+  unfolding box_open_def box_assn_def by vcg
+
+definition box_free :: \<open>('c \<Rightarrow> unit llM) \<Rightarrow> 'c::llvm_rep ptr \<Rightarrow> unit llM\<close> where [llvm_code]:
+  \<open>box_free fr p \<equiv> doM {
+    c \<leftarrow> ll_load p;
+    fr c;
+    ll_free p
+  }\<close>
+
+lemma box_free_rule:
+  assumes [THEN MK_FREED, vcg_rules]: \<open>MK_FREE A fr\<close>
+  shows \<open>MK_FREE (\<upharpoonleft>(box_assn A)) (box_free fr)\<close>
+  apply rule
+  unfolding box_free_def box_assn_def
+  by vcg
+
+subsection \<open>Null test\<close>
+
+context begin
+interpretation llvm_prim_arith_setup .
+
+lemma ll_ptrcmp_eq_null_simp:
+  \<open>ll_ptrcmp_eq a null = doM { Mreturn (from_bool (a = null))}\<close>
+  by (vcg_normalize; simp add: eq_commute[of null])
+
+end
+
+definition box_is_null :: \<open>'c::llvm_rep ptr \<Rightarrow> 1 word llM\<close> where [llvm_code, llvm_inline]:
+  \<open>box_is_null p \<equiv> ll_ptrcmp_eq p null\<close>
+
+lemma box_is_null_rule[vcg_rules]:
+  \<open>llvm_htriple \<box> (box_is_null p) (\<lambda>r. \<upharpoonleft>bool.assn (p = null) r)\<close>
+  unfolding box_is_null_def ll_ptrcmp_eq_null_simp
+  supply [simp] = bool.assn_def
+  by vcg
+
+subsection \<open>The boxed map instance\<close>
+
+locale boxed_pmap =
+  fixes A :: \<open>'a \<Rightarrow> 'c::llvm_rep \<Rightarrow> assn\<close>
+    and fr :: \<open>'c \<Rightarrow> unit llM\<close>
+  assumes Afree: \<open>MK_FREE A fr\<close>
+begin
+
+sublocale array_pmap \<open>null\<close> \<open>\<upharpoonleft>(box_assn A)\<close> box_is_null \<open>box_free fr\<close>
+  apply unfold_locales
+  subgoal by simp
+  subgoal by (rule box_is_null_rule)
+  subgoal by simp
+  subgoal by (rule box_free_rule[OF Afree])
+  done
+
+end
+
+section \<open>Copying Partial Maps\<close>
+text \<open>Our previous map did not assume that container elements can be copied.
+  This implies that extracting function (like lookup) will move ownership out of the map.
+  If we assume that elements can be copied, we can also provide an alternative variant
+  were the map is kept intact and the caller isn't required to reassemble it.\<close>
+
+locale copying_array_pmap = array_pmap +
+  fixes acopy :: \<open>'a \<Rightarrow> 'a llM\<close>
+  assumes acopy_is_copy: \<open>is_copy A acopy\<close>
+begin
+
+sublocale copy_free_context A afree acopy 
+  apply unfold_locales
+  by (simp_all add: Afree GEN_ALGO_def acopy_is_copy)
+
+definition[llvm_inline]: \<open>copy_option cp c \<equiv> doM { d \<leftarrow> is_dflt c; llc_if d (Mreturn c) (cp c) } \<close>
+
+lemma copy_option_rule[vcg_rules]:
+  \<open>llvm_htriple
+     (option_assn a c)
+     (copy_option acopy c)
+     (\<lambda>r. option_assn a c ** option_assn a r)\<close>
+  supply [vcg_rules] = CMP
+  supply [simp] = option_assn_None_conv UU
+  unfolding copy_option_def
+  apply (cases a; simp)
+  apply vcg
+  done
+
+lemma pmap_copy_slot_rule[vcg_rules]:
+  \<open>llvm_htriple
+     (\<upharpoonleft>(list_assn (mk_assn option_assn)) xs xsi ** \<up>\<^sub>d(i < length xs))
+     (copy_option acopy (xsi ! i))
+     (\<lambda>r. \<upharpoonleft>(list_assn (mk_assn option_assn)) xs xsi ** option_assn (xs ! i) r)\<close>
+proof (cases \<open>i < length xs\<close>)
+  case True
+  show ?thesis
+    unfolding vcg_tag_defs list_assn_option_focus[OF True]
+    by vcg
+next
+  case False
+  show ?thesis
+    unfolding vcg_tag_defs
+    apply (rule htriple_realizable_preI)
+    using False by (simp add: sep_algebra_simps)
+qed
+
+definition cpmap_lookup :: \<open>64 word \<Rightarrow> 'a pmap_conc \<Rightarrow> 'a llM\<close> where[llvm_code]:
+  \<open>cpmap_lookup ii ai \<equiv> doM {
+    l \<leftarrow> arl_len ai;
+    b \<leftarrow> ll_icmp_ult ii l;
+    llc_if b (doM {
+      \<comment> \<open>We just hope/assume that clang will optimize this\<close>
+      a \<leftarrow> arl_nth ai ii;
+      a2 \<leftarrow> copy_option acopy a;
+      arl_upd ai ii a2;
+      Mreturn a
+    })
+    (Mreturn init)
+  }\<close>
+
+lemma cpmap_lookup_reassemble_hit:
+  assumes A: \<open>i < length xsi\<close>
+  shows \<open>ENTAILS
+    (\<upharpoonleft>iarl_assn (xsi[i := rb]) ai **
+     \<upharpoonleft>(list_assn (mk_assn option_assn)) xs xsi **
+     option_assn (xs ! i) rb)
+    ((EXS z. \<upharpoonleft>iarl_assn z ai ** \<upharpoonleft>(list_assn (mk_assn option_assn)) xs z)
+     ** option_assn (if i < length xs then xs ! i else Option.None) (xsi ! i))\<close>
+proof (cases \<open>length xs = length xsi\<close>)
+  case True
+  with A have K: \<open>i < length xs\<close> by simp
+  show ?thesis
+    unfolding ENTAILS_def
+    apply (simp add: A K list_assn_option_focus[OF K] sep_conj_exists)
+    apply (rule entails_exI[where x=\<open>xsi[i := rb]\<close>])
+    by (simp add: A sep_conj_aci)
+next
+  case False
+  then show ?thesis
+    unfolding ENTAILS_def by (auto simp: entails_def sep_algebra_simps)
+qed
+
+lemma cpmap_lookup_reassemble_miss:
+  assumes A: \<open>\<not> i < length xsi\<close>
+  shows \<open>ENTAILS
+    (\<upharpoonleft>iarl_assn xsi ai ** \<upharpoonleft>(list_assn (mk_assn option_assn)) xs xsi)
+    ((EXS z. \<upharpoonleft>iarl_assn z ai ** \<upharpoonleft>(list_assn (mk_assn option_assn)) xs z)
+     ** option_assn (if i < length xs then xs ! i else Option.None) init)\<close>
+proof (cases \<open>length xs = length xsi\<close>)
+  case True
+  with A have K: \<open>\<not> i < length xs\<close> by simp
+  show ?thesis
+    unfolding ENTAILS_def
+    apply (simp add: K dflt_is_init[symmetric] sep_algebra_simps)
+    apply (rule entails_exI[where x=xsi])
+    by (simp add: sep_conj_aci)
+next
+  case False
+  then show ?thesis
+    unfolding ENTAILS_def by (auto simp: entails_def sep_algebra_simps)
+qed
+
+lemma cpmap_lookup_rule[vcg_rules]:
+  \<open>llvm_htriple
+    (\<upharpoonleft>snat.assn i ii ** pmap_assn' xs ai)
+    (cpmap_lookup ii ai)
+    (\<lambda>r. pmap_assn' xs ai ** option_assn (opt_list_lookup i xs) r)\<close>
+  unfolding cpmap_lookup_def opt_list_lookup_def
+  supply [simp] = pmap_assn_def
+  apply vcg
+  subgoal by (rule cpmap_lookup_reassemble_hit)
+  apply vcg
+  subgoal by (rule cpmap_lookup_reassemble_miss)
+  done
+
+lemma cpmap_lookup_hnr:
+  \<open>(uncurry cpmap_lookup, uncurry (RETURN oo opt_list_lookup))
+  \<in> (snat_assn' TYPE(64))\<^sup>k *\<^sub>a pmap_assn'\<^sup>k \<rightarrow>\<^sub>a option_assn\<close>
+  unfolding snat_rel_def snat.assn_is_rel[symmetric]
+  apply sepref_to_hoare
+  by vcg
+
+lemmas cpmap_lookup_hnr2[sepref_fr_rules] =
+  cpmap_lookup_hnr[FCOMP opt_list_lookup_refine]
+
+lemma opt_list_the_lookup_conv:
+  \<open>opt_list_contains_key k m \<Longrightarrow> opt_list_lookup k m = Option.Some (opt_list_the_lookup k m)\<close>
+  unfolding opt_list_contains_key_def opt_list_lookup_def opt_list_the_lookup_def
+  by (auto split: if_splits)
+
+lemma cpmap_the_lookup_hnr:
+  \<open>(uncurry cpmap_lookup, uncurry (RETURN oo opt_list_the_lookup))
+  \<in> [\<lambda>(k,xs). opt_list_contains_key k xs]\<^sub>a (snat_assn' TYPE(64))\<^sup>k *\<^sub>a pmap_assn'\<^sup>k \<rightarrow> A\<close>
+  unfolding snat_rel_def snat.assn_is_rel[symmetric]
+  supply [simp] = opt_list_the_lookup_conv
+  by (sepref_to_hoare; vcg)
+
+lemmas cpmap_the_lookup_hnr2[sepref_fr_rules] =
+  cpmap_the_lookup_hnr[FCOMP opt_list_the_lookup_refine]
+
+end
+
+section \<open>Experiments\<close>
+
+text \<open>Sanity tests: instantiate the copying map with boxed 64-bit numbers
+  (a \<open>nat \<rightharpoonup> nat\<close> map at the HOL level) and let sepref synthesize small test
+  programs written against the IICF map interface. This exercises the registered
+  \<open>sepref_fr_rules\<close> (empty/update/delete/contains\_key/lookup/the\_lookup) and the
+  frame free rules (\<open>pmap_free\<close>, lifted through \<open>hr_comp\<close> by @{thm MK_FREE_hrcompI}).\<close>
+
+experiment
+begin
+
+text \<open>A copy function for boxes with pure content: load and re-allocate.\<close>
+definition box_copy :: \<open>'c::llvm_rep ptr \<Rightarrow> 'c ptr llM\<close> where [llvm_code, llvm_inline]:
+  \<open>box_copy p \<equiv> doM { c \<leftarrow> ll_load p; ll_ref c }\<close>
+
+lemma box_copy_pure_rule[vcg_rules]:
+  \<open>llvm_htriple
+    (\<upharpoonleft>(box_assn (pure R)) x p)
+    (box_copy p)
+    (\<lambda>r. \<upharpoonleft>(box_assn (pure R)) x p ** \<upharpoonleft>(box_assn (pure R)) x r)\<close>
+  unfolding box_copy_def box_assn_def
+  supply [simp] = pure_app_eq
+  by vcg
+
+lemma box_copy_hnr:
+  \<open>(box_copy, RETURN o COPY) \<in> (\<upharpoonleft>(box_assn (pure R)))\<^sup>k \<rightarrow>\<^sub>a \<upharpoonleft>(box_assn (pure R))\<close>
+  apply sepref_to_hoare
+  apply (fold pure_def)
+  by vcg
+
+interpretation P: copying_array_pmap
+  null \<open>\<upharpoonleft>(box_assn (snat_assn' TYPE(64)))\<close> box_is_null
+  \<open>box_free (\<lambda>_. Mreturn ())\<close> box_copy
+  apply unfold_locales
+  subgoal by simp
+  subgoal by (rule box_is_null_rule)
+  subgoal by simp
+  subgoal by (rule box_free_rule[OF mk_free_pure])
+  subgoal unfolding is_copy_def by (rule box_copy_hnr)
+  done
+
+text \<open>Boxing is an implementation detail invisible at the HOL level; to move values
+  into/out of the map, sepref needs named identity ops with box conversion rules.\<close>
+definition BOX :: \<open>'v \<Rightarrow> 'v\<close> where \<open>BOX x \<equiv> x\<close>
+definition UNBOX :: \<open>'v \<Rightarrow> 'v\<close> where \<open>UNBOX x \<equiv> x\<close>
+sepref_register BOX UNBOX
+
+lemma BOX_hnr[sepref_fr_rules]:
+  \<open>(box_new, RETURN o BOX)
+    \<in> (snat_assn' TYPE(64))\<^sup>d \<rightarrow>\<^sub>a \<upharpoonleft>(box_assn (snat_assn' TYPE(64)))\<close>
+  supply [simp] = invalid_pure_recover pure_app_eq refine_pw_simps
+  apply sepref_to_hoare
+  apply (fold pure_def)
+  unfolding BOX_def box_new_def box_assn_def
+  by vcg
+
+lemma UNBOX_hnr[sepref_fr_rules]:
+  \<open>(box_open, RETURN o UNBOX)
+    \<in> (\<upharpoonleft>(box_assn (snat_assn' TYPE(64))))\<^sup>d \<rightarrow>\<^sub>a snat_assn' TYPE(64)\<close>
+  supply [simp] = invalid_pure_recover pure_app_eq refine_pw_simps invalid_assn_def
+  apply sepref_to_hoare
+  apply (fold pure_def)
+  unfolding UNBOX_def box_open_def box_assn_def
+  by vcg
+
+(* BISECT2: tests disabled
+text \<open>Insert, query, delete \<emdash> the map lives and dies inside the program, so this
+  also tests the synthesized free (\<open>pmap_free\<close> with per-slot \<open>box_free\<close>).\<close>
+sepref_definition pmap_test1_impl is
+  \<open>uncurry (\<lambda>k v. do {
+      let m = op_map_empty;
+      let m = op_map_update k (BOX v) m;
+      let b\<^sub>1 = op_map_contains_key k m;
+      let m = op_map_delete k m;
+      let b\<^sub>2 = op_map_contains_key k m;
+      RETURN (b\<^sub>1 \<and> \<not> b\<^sub>2)
+    })\<close>
+  :: \<open>[\<lambda>(k, v). k + 1 < max_snat 64]\<^sub>a
+      (snat_assn' TYPE(64))\<^sup>k *\<^sub>a (snat_assn' TYPE(64))\<^sup>k \<rightarrow> bool1_assn\<close>
+  by sepref
+
+text \<open>Round-trip a value through the map (guarded lookup, key present by construction).\<close>
+sepref_definition pmap_test2_impl is
+  \<open>uncurry (\<lambda>k v. do {
+      let m = op_map_update k (BOX v) op_map_empty;
+      let x = op_map_the_lookup k m;
+      RETURN (UNBOX x)
+    })\<close>
+  :: \<open>[\<lambda>(k, v). k + 1 < max_snat 64]\<^sub>a
+      (snat_assn' TYPE(64))\<^sup>k *\<^sub>a (snat_assn' TYPE(64))\<^sup>k \<rightarrow> snat_assn' TYPE(64)\<close>
+  by sepref
+
+*)
+text \<open>The optional lookup, returning the option itself.\<close>
+(* TEMPORARILY DISABLED (bisecting a hang)
+sepref_definition pmap_test3_impl is
+  \<open>uncurry (\<lambda>k v. do {
+      let m = op_map_update k (BOX v) op_map_empty;
+      RETURN (op_map_lookup k m)
+    })\<close>
+  :: \<open>[\<lambda>(k, v). k + 1 < max_snat 64]\<^sub>a
+      (snat_assn' TYPE(64))\<^sup>k *\<^sub>a (snat_assn' TYPE(64))\<^sup>k
+      \<rightarrow> hr_comp P.option_assn (\<langle>nat_rel\<rangle>option_rel)\<close>
+  by sepref
+*)
+
+end
 
 end
